CompCert/Events.v
@@ -5,7 +5,8 @@ Require Import CompCert.Coqlib.
 
 Class EventClass (A : Type) :=
   { next_comp_of_event : A -> Component.id;
-    cur_comp_of_event : A -> Component.id
+    cur_comp_of_event : A -> Component.id;
+    event_equal : A -> A -> Prop
   }.
 
 
@@ -20,6 +21,20 @@ Inductive event :=
 | ERet : Component.id -> Z (* value *) -> Component.id -> event
 | ERead : Component.id -> Pointer.t -> value -> event
 | EWrite : Component.id -> Pointer.t -> value -> event.
+
+Inductive match_event : event -> event -> Prop :=
+| match_events_call: forall C P arg C',
+    match_event (ECall C P arg C')
+                (ECall C P arg C')
+| match_events_ret: forall C retval C',
+    match_event (ERet C retval C')
+                (ERet C retval C')
+| match_events_read: forall C ptr v,
+    match_event (ERead C ptr v)
+                (ERead C ptr v)
+| match_events_write: forall C ptr v,
+    match_event (EWrite C ptr v)
+                (EWrite C ptr v).
 
 Instance event_EventClass : EventClass event :=
   {
@@ -38,7 +53,8 @@ Instance event_EventClass : EventClass event :=
       (* Reads and writes retain control. *)
       | ERead  C _ _   => C
       | EWrite C _ _   => C
-      end
+      end;
+    event_equal := match_event
   }.
 
 Definition trace (A : Type) := list A.
@@ -238,10 +254,13 @@ Set Implicit Arguments.
   The name "match_traces" should be changed.
   Maybe it should be "check_both_nil_or_singleton" or similar.
 *)
-Inductive match_traces: (@trace event) -> (@trace event) -> Prop :=
-  | match_traces_E0:
-      match_traces nil nil
-  | match_traces_call: forall C P arg C',
+Inductive equal_and_nil_or_singleton
+          {Ev} {evInst: EventClass Ev} : (trace Ev) -> (trace Ev) -> Prop :=
+| match_traces_E0:
+    equal_and_nil_or_singleton nil nil
+| match_traces_singleton: forall e e',
+    event_equal e e' -> equal_and_nil_or_singleton (e :: nil) (e' :: nil).
+(*  | match_traces_call: forall C P arg C',
       match_traces (ECall C P arg C' :: nil)
                    (ECall C P arg C' :: nil)
   | match_traces_ret: forall C retval C',
@@ -253,3 +272,4 @@ Inductive match_traces: (@trace event) -> (@trace event) -> Prop :=
   | match_traces_write: forall C ptr v,
       match_traces (EWrite C ptr v :: nil)
                    (EWrite C ptr v :: nil).
+*)
